\documentclass[12pt]{article}

\begin{document}

\textit{Proposed Solution to \#5729 SSMJ }\\ \\
\textit{Solution proposed by Prakash Pant, Mathematics Initiatives in Nepal, Bardiya, Nepal.}\\ \\
\textit{Problem proposed by Goran Conar, Varazdin, Croatia.} \\ \\
\textbf{Statement of the Problem:}
 Let $0<a<b$ be real numbers. Prove the following inequality:\\
\[ (a+b)^{(a+b)} (b-a)^{(b-a)} < (\frac{a^2 + b^2}{b})^{2b}  \]


\textbf{Solution of the Problem:} 		d			
We modify the problem taking ln on both sides, \\
\[ 	(a+b)\ln(a+b)+(b-a)\ln(b-a) < 2b \ln(\frac{a^2+b^2}{b})	 \hspace{1cm} ...........(1)				\]
Now, we will focus on proving this statement. \\ \\ 
Then, consider a function $ f(x) =  \ln(x)$. Then f''(x) = $-\frac{1}{x^2}<0$ $\forall x>0 $. So, the function is concave $\forall x \neq 0$. Also notice that both a+b and b-a are strictly positive here.  \\
Now, using Jensen's inequality,\\
\[  \frac{(a+b) \ln(a+b)+(b-a)\ln(b-a)}{a+b+b-a} \le \ln(\frac{(a+b)(a+b)+(b-a)(b-a)}{a+b+b-a})		\]		
which on simplification gives 
\[(a+b)\ln(a+b)+(b-a)\ln(b-a) \le 2b \ln(\frac{a^2+b^2}{b})						\]	
And the equality holds when $ a+b = b-a$ $\Rightarrow$ a=0. But since $0<a<b$, the equality does not hold. Hence, we have proved (1).
					


\end{document}