\documentclass[12pt]{article}

\begin{document}

\textit{Proposed Solution to \#5738 SSMJ }\\ \\
\textit{Solution proposed by Prakash Pant, Mathematics Initiatives in Nepal, Bardiya, Nepal.}\\ \\
\textit{Problem proposed by Goran Conar, Varazdin, Croatia.} \\ \\
\textbf{Statement of the Problem:}
 Let $x_1,......x_n >0 $  be real numbers and $s = \sum_{i=1}^{n} x_i $. Prove \\
\[ \prod_{i=1}^{n} x_i^{x_i} \ge  (\frac{s}{n+s})^s \prod_{i=1}^{n} {(1+x_i)}^{x_i}.	\]
When does equality occur? \\ \\ 

\textbf{Solution of the Problem:}
We first rearrange the problem as follows:\\
\[ \prod_{i=1}^{n} (\frac{x_i}{1+x_i})^{x_i}\ge  (\frac{s}{n+s})^s  					\]
We further modify the problem taking log on both sides, \\
\[ \sum_{i=1}^{n} x_i \ln(\frac{x_i}{1+x_i})	\ge s \ln(\frac{s}{n+s}) \hspace{1cm} ...........(1)				\]
Now, we will focus on proving this statement. \\ \\ 
Then, consider a function $ f(x) = x \ln (\frac{x}{1+x})$. Then f''(x) = $\frac{1}{x(1+x)^2}>0$ $\forall x>0 $. So, the function is convex in our required interval. \\
Now, using Jensen's inequality,\\
\[	\frac{\sum_{i=1}^{n} x_i \ln(\frac{x_i}{1+x_i})}{n}	\ge \frac{\sum_{i=1}^{n} x_i}{n} 
\ln(\frac{ \frac{\sum_{i=1}^{n} x_i}{n}}{1 + \frac{\sum_{i=1}^{n} x_i}{n}} )						\]		
which on simplification gives
\[	\sum_{i=1}^{n} x_i \ln(\frac{x_i}{1+x_i})\ge s
\ln(\frac{s}{n+s} )						\]	
which is what was to be proved from (1). And the equality holds when $ x_1 = x_2 = ....=x_n .$
					


\end{document}