\documentclass[12pt]{article}
\usepackage{amsmath}
\begin{document}

\textit{Proposed Solution to \#5768 SSMJ }\\ \\
\textit{Solution proposed by Prakash Pant, Mathematics Initiatives in Nepal, Bardiya, Nepal.}\\ \\
\textit{Proposed by Vasile Mircea Popa, Lucian Blaga University, Sibiu, Romania.} \\ \\
\textbf{Statement of the Problem:}
\[ \text{ Calculate the integral} : \]
\[ I = \int_0^{\infty} \frac{\arctan(x) \ln^2(x)}{x^2+x+1} dx\]

\textbf{Solution of the Problem:}
\[ I_1 = \int_0^{\infty} \frac{\arctan(x) \ln^2(x)}{x^2+x+1} dx\]
Substitute x by 1/x, we get
\[ I_2 = \int_{\infty}^{0} \frac{ \arctan(1/x) (-\ln(x))^2}{1+x+x^2}x^2 . \frac{-1}{x^2} dx = \int_0^{\infty} \frac{arccot(x) \ln^2(x)}{x^2+x+1} dx \]
Adding $I_1$ and $I_2$ and using the property that $\arctan(x)$+arccot(x) = $\frac{\pi}{2}$ ,
\[ 2I = \int_0^{\infty} \frac{(\arctan(x)+ arccot(x)) \ln^2(x)}{x^2+x+1} =\frac{\pi}{2} \int_0^{\infty} \frac{ \ln^2(x)}{x^2+x+1}  dx\]

\[ \text{ Now, to find}  \int_0^{\infty} \frac{ \ln^2(x)}{x^2+x+1}  dx , \text{ we solve the integral J(a) }= \int_0^{\infty} \frac{x^a}{x^2+x+1}dx ,\]\[ \text{ and then calculate  J''(0) }\] 
\[ J(a) =  \int_0^1 \frac{x^a}{x^2+x+1}dx + \int_1^{\infty} \frac{x^a}{x^2+x+1}dx  \]
Substituting x as 1/x in the second integral 
\[ J(a) =  \int_0^1 \frac{x^a}{x^2+x+1}dx + \int_1^0 \frac{x^{-a}}{1+x+x^2}x^2 . \frac{-1}{x^2} dx =  \int_0^1 \frac{x^a + x^{-a}}{x^2+x+1}dx  \]
\[ Further, J(a) =  \int_0^1 \frac{(x^a + x^{-a})(1-x)}{1-x^3}dx \]
Substitute x as $x^{\frac{1}{3}}$,
\[  J(a) =  \int_0^1 \frac{(x^{\frac{a}{3}} + x^{\frac{-a}{3}})(1-x^{\frac{1}{3}})}{1-x} \frac{x^{\frac{-2}{3}}}{3} dx  = \frac{1}{3} \int_0^1 \frac{ x^{\frac{a-2}{3}} + x^{\frac{-a-2}{3}} - x^{\frac{a-1}{3}} - x^{\frac{-a-1}{3}}  }{1-x}  dx \]

\[  J(a) = \frac{1}{3} \int_0^1 \frac{1- x^{\frac{-a-1}{3}} }{1-x} + \frac{1- x^{\frac{a-1}{3}}}{1-x} - \frac{1- x^{\frac{a-2}{3}} }{1-x}- \frac{1- x^{\frac{-a-2}{3}} }{1-x}   dx \]

Using $ \psi (a+1) + \gamma = \int_0^1 \frac{1-x^a}{1-x} dx $, where $\gamma$ is euler mascheroni constant, 
\[  J(a) = \frac{1}{3} \left[   \psi\left( \frac{-a+2}{3} \right) + \psi \left( \frac{a+2}{3} \right) - \psi\left( \frac{a+1}{3} \right) - \psi \left( \frac{-a+1}{3} \right)   \right] \]

\[  J(a) = \frac{1}{3} \left[    \psi\left( 1- \frac{a+1}{3} \right) - \psi\left( \frac{a+1}{3} \right) - \left[ \psi\left(1- \frac{a+2}{3}\right) -   \psi\left( \frac{a+2}{3}\right)      \right] \right] \]
Using the reflection property of digamma function, $ \psi(1-x)-\psi(x) = \pi \cot(\pi x )} $ ,
\[  J(a) = \frac{1}{3} \left[ \pi\cot(\pi (\frac{a+1}{3})) - \pi\cot(\pi (\frac{a+2}{3})) \right]  \]

\[ J'(a) = \frac{\pi}{3} \left[ -cosec^2(\pi (\frac{a+1}{3})) \frac{\pi}{3} + cosec^2(\pi (\frac{a+2}{3})) \frac{\pi}{3} \right] \]

\[ J''(a) = \frac{\pi^2}{9} \left[ (-2cosec(\pi (\frac{a+1}{3}))) (-cosec(\pi (\frac{a+1}{3}))cot(\pi (\frac{a+1}{3})))\frac{\pi}{3}  +\]\[ (2cosec(\pi (\frac{a+2}{3}))) (-cosec(\pi (\frac{a+2}{3}))cot(\pi (\frac{a+2}{3})))\frac{\pi}{3} \Big] \]

\[ J''(0) = \frac{2 \pi^3}{27} \left[ \frac{2}{\sqrt{3}}. \frac{2}{\sqrt{3}}. \frac{1}{\sqrt{3}} - \frac{2}{\sqrt{3}}. \frac{2}{\sqrt{3}}. \frac{-1}{\sqrt{3}} \right] \]
 
\[ J''(0) = \frac{16 \pi^3}{81 \sqrt{3}}\]
\[ \text{ Using 2I = }\frac{\pi}{2} J''(0)\text{, we get I = }\frac{\pi}{4} \times \frac{16 \pi^3}{81 \sqrt{3}} = \frac{4 \pi^4}{81 \sqrt{3}} \] 



\end{document}