\documentclass[12pt]{article}
\usepackage{amsmath}
\begin{document}

\textit{Proposed Solution to \#5773 SSMJ }\\ \\
\textit{Solution proposed by Prakash Pant, Mathematics Initiatives in Nepal, Bardiya, Nepal.}\\ \\
\textit{Proposed by Vasile Mircea Popa, Lucian Blaga University, Sibiu, Romania.} \\ \\
\textbf{Statement of the Problem:}
\[ \text{ Calculate the following integral} : \]
\[ I = \int_0^{1}  \frac{x \ln^2(x)}{x^3+x\sqrt{x}+1} dx\]

\textbf{Solution of the Problem:}
\[ I = \int_0^{1}  \frac{x \ln^2(x)}{(x^{\frac{3}{2}})^2+x^{\frac{3}{2}}+1} dx \]
Multiplying numerator and denominator by $(1-x^{\frac{3}{2}})$,
 \[ I = \int_0^{1}  \frac{x \ln^2(x)(1-x^{\frac{3}{2}})}{(1-x^{\frac{9}{2}})}  dx \]
Since $|x^{\frac{9}{2}}|<1 $ as x goes from 0 to 1 , we can use infinite geometric series expansion, 
 \[ I = \int_0^{1} x \ln^2(x)(1-x^{\frac{3}{2}})\sum_{n=0}^{\infty} x^{\frac{9n}{2}}  dx \]
Taking constants inside the sum and interchanging sum and interval using dominated convergence theorem,
 \[ I = \sum_{n=0}^{\infty} \int_0^{1}  x \ln^2(x)(1-x^{\frac{3}{2}}) x^{\frac{9n}{2}}  dx = \sum_{n=0}^{\infty}   \int_0^{1}  \left( \ln^2(x) x^{\frac{9n}{2}+1} - \ln^2(x)x^{\frac{9n}{2}+\frac{5}{2}} \right)  dx\]

 Using $\int_0^1 \ln^n(x)x^m dx = (-1)^n \frac{\Gamma(n+1)}{(m+1)^{n+1}}$ ,
 \[ I = \sum_{n=0}^{\infty} \frac{\Gamma(3)}{(\frac{9n}{2}+2)^3} - \frac{\Gamma(3)}{(\frac{9n}{2}+\frac{7}{2})^3} = \frac{8}{729} \sum_{n=0}^{\infty} \frac{2}{(n+\frac{4}{9})^3} - \frac{2}{(n+\frac{7}{9})^3} \] 
 Using $\psi''(x)= \sum_{n=0}^{\infty} \frac{-2}{(n+x)^3} $,
 \[ I  = \frac{8}{729} \left( \psi''(\frac{7}{9})- \psi''(\frac{4}{9}) \right) = 0.20744 \]  













\end{document}