\documentclass[12pt]{article}
\usepackage{amsmath}
\begin{document}

\textit{Proposed Solution to \#U649 Undergraduate Problems, Mathematical Reflections 1 (2024) }\\ \\
\textit{Solution proposed by Prakash Pant, Mathematics Initiatives in Nepal, Bardiya, Nepal.}\\ \\
\textit{Problem Proposed by by Mircea Becheanu, Canada} \\ \\
\textbf{Statement of the Problem:}
\[ \text{ Evaluate} : \]
\[ \lim_{n \to \infty} \left(  \frac{(1^2+n^2)(2^2+n^2)...(n^2+n^2)}{n!n^n} \right) ^{\frac{1}{n}} \]

\textbf{Solution of the Problem:} \\
Let L be the limit,
\[ L = \lim_{n \to \infty} \left(  \frac{(1^2+n^2)(2^2+n^2)...(n^2+n^2)}{n!n^n} \right) ^{\frac{1}{n}} = \lim_{n \to \infty} \left(  \prod_{k=1}^{n} \frac{k^2+n^2}{kn} \right)^{\frac{1}{n}} \]
Taking log on both sides,
\[ \log(L) = \lim_{n \to \infty} \frac{1}{n} \sum_{k=1}^n \log \left( \frac{k^2+n^2}{kn} \right) = \lim_{n \to \infty}  \sum_{k=1}^n \frac{1}{n} \log \left( \frac{k}{n} + \frac{n}{k} \right)           \]
We know $\lim_{n \to \infty}  \sum_{k=1}^n \left[ f(a+ \frac{(b-a)}{n}k)\frac{b-a}{n} \right] = \int_a^b f(x) dx $ ,Thus
\[ \log(L) =  \lim_{n \to \infty}  \sum_{k=1}^n \frac{1}{n} \log \left( \frac{k}{n} + \frac{n}{k} \right) = \int_0^1 \log(x+\frac{1}{x}) dx  = \int_0^1 \log(x^2+1) dx - \int_0^1 \log(x) dx       \]
Using integration by parts for the first integral,
\[I_1= \int_0^1 \log(x^2+1) dx = \log(x^2+1) x \Big|_0^1 - 2\int_0^1 \frac{x^2}{x^2+1} dx = \log(x^2+1) x \Big|_0^1 - 2\int_0^1 \left( 1- \frac{1}{x^2+1} \right) dx \]
\[I_1 = \log(x^2+1) x \Big|_0^1 - 2\int_0^1 1 dx + \int_0^1 \frac{2}{x^2+1} dx   \]
\[I_1 = \log(x^2+1) x \Big|_0^1 - 2x\Big|_0^1 + 2\arctan(x)\Big|_0^1  = \log(2)-2+\frac{\pi}{2}  \]
Using integration by parts for the second integral as well,
\[I_2 = \int_0^1 \log(x) dx = (x \log(x)-x)\Big|_0^1 = -1 \]
Combining,
\[ \log(L) =I_1-I_2= \log(2)-2+\frac{\pi}{2} - (-1) = \log(2)+\frac{\pi}{2}-1 \] 
\[  L = 2 e^{ \frac{\pi}{2}-1 \]















\end{document}