\documentclass[12pt]{article}
\usepackage{amsmath}
\begin{document}

\textit{Proposed Solution to \#U650 Undergraduate Problems, Mathematical Reflections 1 (2024) }\\ \\
\textit{Solution proposed by Prakash Pant, Mathematics Initiatives in Nepal, Bardiya, Nepal.}\\ \\
\textit{Problem Proposed by  by Mihaela Berindeanu, Bucharest, Rom√¢nia.} \\ \\
\textbf{Statement of the Problem:}
\[ \text{ Evaluate} : \]
\[ I = \int_1^e \frac{(\ln(x)-1)^2-3}{(\ln(x)+2)^2} dx\]

\textbf{Solution of the Problem:} \\
Substitute $ \ln(x)$ as x , 
\[ I = \int_0^1 \frac{(x-1)^2-3}{(x+2)^2} e^x dx\]
\[ I = \int_0^1 \frac{(x+2-3)^2-3}{(x+2)^2} e^x dx\]
\[ I = \int_0^1 \frac{(x+2)^2-6(x+2)+9-3}{(x+2)^2} e^x dx\]
\[ I = \int_0^1 \left[ e^x - \frac{6 e^x}{(x+2)} + \frac{6 e^x}{(x+2)^2} \right] dx \]
\[ I = \int_0^1  e^x dx - \int_0^1  \frac{6 e^x}{(x+2)} dx +\int_0^1 \frac{6 e^x}{(x+2)^2}  dx \]
Using integration by parts in third integral,
\[\int_0^1 \frac{6 e^x}{(x+2)^2}  dx =  -  \frac{6e^x}{(x+2)}\Big|_0^1 +  \int_0^1 \frac{6 e^x}{(x+2)}  dx \]
Thus, 
\[ I = \int_0^1  e^x dx - \int_0^1  \frac{6 e^x}{(x+2)} dx -  \frac{6e^x}{(x+2)}\Big|_0^1 +  \int_0^1 \frac{6 e^x}{(x+2)}    dx \]
\[ I =  e^x \Big|_0^1  -  \frac{6e^x}{(x+2)}\Big|_0^1     dx \]
\[ I =  (e-1)  -  (2e-3)   = 2-e  \text{, which is the answer.} \]




\end{document}